{
 "cells": [
  {
   "cell_type": "markdown",
   "metadata": {},
   "source": [
    "## Практическое задание к уроку 5"
   ]
  },
  {
   "cell_type": "markdown",
   "metadata": {},
   "source": [
    "### Тема “Предел функции” [link](https://docs.google.com/document/d/1tvR4TDHjKiNhO5E6iO-AUuklb1HWY8IFjRzsW2m1Utc/edit)\n",
    "\n",
    "4. \n",
    "### $$а)\\,\\,\\,\\,\\lim_{x\\to 0} \\frac{3x^3-2x^2}{4x^2} = \\lim_{x\\to 0} \\frac{x^2(3x-2)}{4x^2} = -\\frac{2}{4} = -\\frac{1}{2}$$\n",
    "### $$б)\\,\\,\\,\\,\\lim_{x\\to 0} \\frac{\\sqrt{1+x} - 1}{\\sqrt[3]{1+x} - 1} = \\lim_{x\\to 0} \\frac{x\\cdot (\\sqrt[3]{(1+x)^2} + \\sqrt[3]{(1+x)} +1)} {x\\cdot (\\sqrt{(1+x)} +1)} = \\frac{\\sqrt[3]{1^2} + \\sqrt[3]{1} + 1}{\\sqrt{1} + 1} = \\frac{3}{2}$$\n",
    "### $$в)\\,\\,\\,\\,\\lim_{x\\to \\infty} \\Bigr(\\frac{x+3}{x}\\Bigl)^{4x+1} = \\lim_{x\\to \\infty} e^ {\\Bigr(\\frac{x+3}{x} - 1\\Bigl) (4x+1)} = \\lim_{x\\to \\infty} e^ {\\frac{x}{3} (4x+1)} = \\lim_{x\\to \\infty} e^ {\\frac{12x+3}{x}} = \\lim_{x\\to \\infty} e^ {12 + \\frac{1}{x}} = e^{12}$$"
   ]
  },
  {
   "cell_type": "markdown",
   "metadata": {},
   "source": [
    "### Тема “Теоремы о пределах” (c-e)\n",
    "\n",
    "### $$c)\\,\\,\\,\\,\\lim_{x\\to 0} \\frac{x}{arcsin(x)} = \\lim_{x\\to 0} (\\frac{arcsin(x)}{x})^{-1} = 1^{-1} = 1$$\n",
    "### $$d)\\,\\,\\,\\,\\lim_{x\\to \\infty} \\Bigl(\\frac{4x+3}{4x-3}\\Bigr)^{6x} = \\lim_{x\\to \\infty} e^{(\\frac{4x+3}{4x-3}-1)6x} = \\lim_{x\\to \\infty} e^{\\frac{(4x+3-4x+3)6x}{4x-3}} = \\lim_{x\\to \\infty} e^{\\frac{(36x}{4x-3}} = e^9$$\n",
    "### $$e)\\,\\,\\,\\,\\lim_{x\\to \\infty} \\frac{sinx+lnx}{x} = \\lim_{x\\to \\infty} \\frac{sinx}{x} + \\lim_{x\\to \\infty} \\frac{lnx}{x} = 0 + 0 = 0$$"
   ]
  },
  {
   "cell_type": "markdown",
   "metadata": {},
   "source": [
    "### Тема 6 “Понятие о производной” [link](https://docs.google.com/document/d/1HRwzoqqSsiC7NFptVi-nxVsiop2xImFENTmrjWxSqGM/edit)\n",
    "\n",
    "### $$a)\\,\\,\\,(sinx\\cdot cosx)' = cos^2x + (-sinx)\\cdot sinx = cos^2x - sin^2x = cos2x$$\n",
    "### $$b)\\,\\,\\,(ln(2x+1)^3)' = \\frac{1 \\cdot 3 \\cdot(2x + 1)^2 \\cdot 2}{(2x + 1)^3} = \\frac{6}{2x+1}$$\n",
    "### $$c)\\,\\,\\,\\Bigl(\\sqrt{sin^2(ln(x^3)})\\Bigr)' = \\frac{1}{2}(sin^2(ln(x^3))^{-\\frac{1}{2}} \\cdot 2sin(ln(x^3)) \\cdot cos(ln(x^3)) \\cdot \\frac{1}{x^3} \\cdot 3x^2 = \\frac{sin(ln(x^3)) \\cdot cos(ln(x^3)) \\cdot 3}{\\sqrt{sin^2(ln(x^3)) \\cdot x}} = \\frac{3cos(ln(x^3))}{x}$$\n",
    "### $$d)\\,\\,\\,\\Bigl(\\frac{x^4}{ln(x)}\\Bigr)' = \\frac{4x^3 \\cdot lnx - \\frac{x \\cdot x^4}{1}}{ln^2x} = \\frac{4x^3 \\cdot lnx - x^5}{ln^2x} = \\frac{4x^3}{lnx} - \\frac{x^3}{ln^2x}$$"
   ]
  }
 ],
 "metadata": {
  "kernelspec": {
   "display_name": "Python 3",
   "language": "python",
   "name": "python3"
  },
  "language_info": {
   "codemirror_mode": {
    "name": "ipython",
    "version": 3
   },
   "file_extension": ".py",
   "mimetype": "text/x-python",
   "name": "python",
   "nbconvert_exporter": "python",
   "pygments_lexer": "ipython3",
   "version": "3.8.6"
  }
 },
 "nbformat": 4,
 "nbformat_minor": 4
}
